\begin{enumerate}
	\item Prove that $ 2\sin^{-1} \brak{\frac{3}{5}} - \tan^{-1} \brak{\frac{17}{31}} = \frac{\pi}{4}$

	\item Solve the equation for $x$: $\cos (\tan^{-1}) = \sin \brak{\cot^{-1} \frac{3}{4}} = \sin \brak{\cot^{-1} \frac{3}{4}}$

	
	\item Solve for 
	\begin{align*}
		x: \tan^{-1}(x-1) + \tan^{-1}x + \tan^{-1}(x+1) = \tan^{-1}3x
	\end{align*}

	\item Prove that 
	\begin{align*}
	\tan^{-1} \brak{\frac{6x-8x^{3}}{1-12x^{2}}} - \tan^{-1} \brak{\frac{4x}{1-4x^{2}}} = \tan^{-1}2x;
	\end{align*}
	\begin{align*}
		\abs{2x} < \frac{1}{\sqrt{3}}
	\end{align*}

	\item The equation of tangent at $\brak{2,3}$ on the curve $y^2 = ax^3 + b$ is $4x -5$. Find the values of $a$ and $b$.
	\item Prove that the curves $y^2 = 4x$ and $x^2 = 4y$ divide the area of square bounded by $x=0, x=4, y=4$ and $y=0$ into three equal parts.
	\item Find the equation of the tangent line to the curve $y = \sqrt{5x - 3} - 5$, which is parallel to the line $4x - 2y + 5 = 0$.
 	\item Prove that 
	\begin{align*}
		2\sin^{-1}\brak{\frac{3}{5}}-\tan^{-1}\brak{\frac{17}{31}} = \frac{\pi}{4}
	\end{align*}
	\item Solve the equation for x:
	\begin{align*}
	\cos\brak{\tan^{-1}x} = \sin\brak{\cot^{-1}\frac{3}{4}}
	\end{align*}

