\begin{enumerate}
\item The roots of the quadratic equation  $2x^2 - x - 6 = 0$ are 
\begin{enumerate}
\item $-2,\dfrac{3}{2}$ 
\item $2,-\dfrac{3}{2}$ 
\item $-2,-\dfrac{3}{2}$ 
\item $2,\dfrac{3}{2}$ 
\end{enumerate}
\item If $1$ is a root of the equations $ay^2 + ay + 3 = 0$ and $y^2 + y + b = 0$, then $ab$ equals : 
\begin{enumerate}
\item $3$ 
\item $-\dfrac{7}{2}$ 
\item $6$ 
\item $-3$ 
\end{enumerate}
\item If the quadratic equation $mx^2 + 2x + m = 0$ has two equal roots, then the values of $m$ are : 
\begin{enumerate}
\item $\pm 1$ 
\item $0,2$ 
\item $0,1$ 
\item $-1,0$ 
\end{enumerate}
%algebra
\item Find the value of $p$ for which the roots of the equation $px\brak{x-2} + 6 = 0$, are equal. 
%Algebra
\item Solve the following quadratic equation for $x$ : 
\begin{align}
x^2 - 4 a x - b^2 + 4a^2 = 0 
\end{align}
%algebra
%algebra
\item Find the value$\brak{\text{s}}$ of $k$ so that the quadratic equation $x^2 - 4kx + k = 0$ has equal roots. 
%algebra
\item Solve for $x$: $4x^2 - 4ax + \brak{a^2 - b^2} = 0$ 
%algebra
\item Solve for $x$: $3x^2 - 2\sqrt 6 x + 2 = 0$ 

\item Find the value of $k$ for which the roots of the quadratic equation $\brak{k - 4} x^2 + 2\brak{k-4} x + 2 =0$ are equal. 
\item Solve for x: 
$4\sqrt 3 x^2 + 5x - 2\sqrt 3 = 0$ 
\end{enumerate}
